minuska/lib/miskeleton.ml
@@ -2,9 +2,57 @@ open Core
 open Printf
 
 
+let ascii_to_char = (fun (b0,b1,b2,b3,b4,b5,b6,b7) ->
+  let f b i = if b then 1 lsl i else 0 in
+  Stdlib.Char.chr (f b0 0 + f b1 1 + f b2 2 + f b3 3 + f b4 4 + f b5 5 + f b6 6 + f b7 7)
+)
+
+let char_to_ascii = (fun c ->
+  let n = Stdlib.Char.code c in
+  let h i = (n land (1 lsl i)) <> 0 in
+  Dsm.Ascii ((h 0), (h 1), (h 2), (h 3), (h 4), (h 5), (h 6), (h 7)))
+
+let rec ascii_list_to_string l =
+  match l with
+  | [] -> Dsm.EmptyString
+  | x::xs -> Dsm.String (x, (ascii_list_to_string xs))
+
+let rec dsmString_to_ascii_list s =
+  match s with
+  | Dsm.EmptyString -> []
+  | Dsm.String (x, xs) -> x::(dsmString_to_ascii_list xs)
+
+let explode' s =
+  let rec exp i l =
+    if i < 0 then l else exp (i - 1) (s.[i] :: l) in
+  (exp (String.length s - 1) [])
+
+let explode s : Dsm.string = ascii_list_to_string (List.map ~f:(char_to_ascii) (explode' s))
+
+let destrut_ascii a =
+  match a with
+  | Dsm.Ascii (b1,b2,b3,b4,b5,b6,b7,b8) ->
+    (b1,b2,b3,b4,b5,b6,b7,b8)
+
+let string_of_chars chars = 
+  let buf = Buffer.create 16 in
+  List.iter ~f:(Buffer.add_char buf) chars;
+  Buffer.contents buf
+
+let implode (s : Dsm.string) : string =
+  let l2 = dsmString_to_ascii_list s in
+  let l3 = List.map ~f:destrut_ascii l2 in
+  let l4 = List.map ~f:(ascii_to_char) l3 in
+  string_of_chars l4
+
+
+
 let convert_builtin (b : Syntax.builtin) : (Dsm.myBuiltinType) =
   match b with
   | `BuiltinInt n -> (Dsm.Bv_Z n)
+  | `BuiltinString s -> (Dsm.Bv_str (explode s))
+  | `BuiltinBool b -> (Dsm.Bv_bool b)
+  | `BuiltinError -> (Dsm.Bv_error)
   | `OpaqueBuiltin -> failwith "Cannot convert unknown builtin back into Coq runtime"
 
 let rec convert_groundterm (g : Syntax.groundterm) : Dsm.gT =
@@ -12,22 +60,25 @@ let rec convert_groundterm (g : Syntax.groundterm) : Dsm.gT =
   | `GTb b ->
     Dsm.gt_over (convert_builtin b)
   | `GTerm (`Id s, gs) ->
-    Dsm.T_term (s,(List.map ~f:convert_groundterm gs))
+    Dsm.T_term ((explode s),(List.map ~f:convert_groundterm gs))
 
 let wrap_init (g : Dsm.gT) : Dsm.gT =
-  Dsm.T_term ("builtin.init", [g])
+  Dsm.T_term ((explode "builtin.init"), [g])
 
 let convert_builtin_back (b : Dsm.myBuiltinType) : Syntax.builtin =
   match b with
   | Dsm.Bv_Z n -> `BuiltinInt n
+  | Dsm.Bv_str s -> `BuiltinString (implode s)
+  | Dsm.Bv_bool b -> `BuiltinBool b
+  | Dsm.Bv_error -> `BuiltinError
   | _ -> `OpaqueBuiltin
 
 let rec convert_groundterm_back (g : Dsm.gT) : Syntax.groundterm =
   match g with
   | Dsm.T_over b ->
     `GTb (convert_builtin_back b)
-  | Dsm.T_term ( s, gs) ->
-    `GTerm (`Id s,(List.map ~f:convert_groundterm_back gs))
+  | Dsm.T_term (s, gs) ->
+    `GTerm (`Id (implode s),(List.map ~f:convert_groundterm_back gs))
 
 let rec run_n_steps step max_depth curr_depth gterm =
   if curr_depth >= max_depth then (curr_depth, gterm)
@@ -78,5 +129,7 @@ let command_run step =
      fun () -> run step program depth output_file ())
 
 let main step =
-    Command_unix.run ~version:"1.0" ~build_info:"RWO" (command_run step)
+  Printexc.record_backtrace true;
+    try (Command_unix.run ~version:"1.0" ~build_info:"RWO" (command_run step)) with
+    | Stack_overflow -> (printf "Stack overflow.\n%s" (Printexc.get_backtrace ()));;
 
