minuska/lib/miunparse.ml
@@ -8,12 +8,15 @@ let mymap (f : 'a -> 'b) (g : 'b -> 'b) (l : 'a list)  : 'b list =
 
 let builtin_to_string (b : Syntax.builtin) : string =
   match b with
-  | `BuiltinInt n -> "(@builtin " ^ (string_of_int n) ^ ")"
+  | `BuiltinInt n -> "(@builtin-int " ^ (string_of_int n) ^ ")"
+  | `BuiltinString s -> "(@builtin-string \"" ^ s ^ "\")"
+  | `BuiltinBool b -> "(@builtin-bool " ^ (if b then "true" else "false") ^ "\")"
+  | `BuiltinError -> "(@builtin-error)"
   | `OpaqueBuiltin -> "(@opaque_builtin)"
 
 let rec groundterm_to_string (g : Syntax.groundterm) : string =
   match g with
-  | `GTb b -> "(" ^ (builtin_to_string b) ^ ")"
+  | `GTb b -> "[" ^ (builtin_to_string b) ^ "]"
   | `GTerm (`Id s, gs) ->
     s ^ "[" ^ (String.concat (mymap groundterm_to_string (fun x -> x ^ ", ") gs)) ^ "]"
 
