minuska/lib/minuska_extraction.v
@@ -1,10 +1,10 @@
 Require Extraction.
 Extraction Language OCaml.
-Require Import
+Require Export
   Coq.extraction.Extraction
   Coq.extraction.ExtrOcamlBasic
-  Coq.extraction.ExtrOcamlNativeString
   Coq.extraction.ExtrOcamlZInt
+  Coq.extraction.ExtrOcamlNatInt
 .
 From Coq Require Import String Bool Arith ZArith List.
 
