minuska-examples/m/imp.m
@@ -1,22 +1,44 @@
 @frames: [
   simple(X): c[builtin.cseq [X,REST], STATE]
 ];
-@value(X): (bool.or(z.is(X), term.same_symbol(X, [var[]]))) ;
-@context(HOLE): c[HOLE];
+@value(X): (bool.or(
+   z.is(X),                            bool.or(
+   bool.is(X),                         bool.or(
+   term.same_symbol(X, [unitValue[]]), 
+   bool.false()
+)))) ;
+@context(HOLE): c[HOLE, STATE];
 @strictness: [
   plus of_arity 2 in [0,1],
   minus of_arity 2 in [0,1],
-  assign of_arity 2 in [1]
+  assign of_arity 2 in [1],
+  seq of_arity 2 in [0],
+  ite of_arity 3 in [0],
+  eq  of_arity 2 in [0,1],
+  le  of_arity 2 in [0,1],
+  lt  of_arity 2 in [0,1],
+  neg of_arity 1 in [0]
 ];
 
 
 @rule [init]: builtin.init[X] => c[builtin.cseq[X, builtin.empty_cseq[]], map.empty()] where bool.true();
-@rule [finish]: c[builtin.cseq[X, builtin.empty_cseq[]]] => builtin.result[X] where z.is(X) ;
 
-@rule/simple [plus]: plus[X,Y] => z.plus(X, Y) where bool.and(z.is(X), z.is(Y)) ;
-@rule/simple [minus]: minus[X,Y] => z.minus(X, Y) where bool.and(z.is(X), z.is(Y)) ;
+@rule/simple [aexpr.plus]: plus[X,Y] => z.plus(X, Y) where bool.and(z.is(X), z.is(Y)) ;
+@rule/simple [aexpr.minus]: minus[X,Y] => z.minus(X, Y) where bool.and(z.is(X), z.is(Y)) ;
 
 @rule [var.assign]: c[builtin.cseq[assign[X,V],REST], STATE] => c[builtin.cseq[unitValue[], REST], map.update(STATE, X, V)] where bool.and(term.same_symbol(X, [var[]]), z.is(V)) ;
 @rule [var.lookup]: c[builtin.cseq[X, REST], STATE] => c[builtin.cseq[map.lookup(STATE, X), REST], STATE] where term.same_symbol(X, [var[]]) ;
+
+@rule/simple [stmt.seq]: seq[unitValue[], X] => X where bool.true() ;
+
+@rule/simple [bexpr.eq]: eq[X, Y] => z.eq(X, Y) where bool.and(z.is(X), z.is(Y)) ;
+@rule/simple [bexpr.le]: le[X, Y] => z.le(X, Y) where bool.and(z.is(X), z.is(Y)) ;
+@rule/simple [bexpr.lt]: lt[X, Y] => z.lt(X, Y) where bool.and(z.is(X), z.is(Y)) ;
+@rule/simple [bexpr.neg]: not[X] => bool.neg(X) where bool.is(X) ;
+
+@rule/simple [stmt.ite.true]: ite[B, X, Y] => X where bool.and(bool.is(B), bool.eq(B, bool.true())) ;
+@rule/simple [stmt.ite.false]: ite[B, X, Y] => Y where bool.and(bool.is(B), bool.eq(B, bool.false())) ;
+
+@rule/simple [while.unfold]: while[B, S] => ite[B, seq[S, while[B, S]], unitValue[]] where bool.true() ;
 
 
